

Assignment 2.5

1) Matrix A has $\text{row}_1 + \text{row}_2 = \text{row}_3$

a. $AX = (1, 0, 0)$ cannot have a solution

$$\hookrightarrow \begin{bmatrix} \text{row}_1 \\ \text{row}_2 \\ \text{row}_1 + \text{row}_2 \end{bmatrix} \begin{bmatrix} x_1 \\ x_2 \\ x_3 \end{bmatrix} = \begin{bmatrix} 1 \\ 0 \\ 0 \end{bmatrix} \rightarrow \text{row}_1 \cdot x_1 + \text{row}_2 \cdot x_2 = 1 + 0 = 1$$

because row 3 supposed to be 1, $AX = (1, 0, 0)$ can't have a solution

b. $A = \begin{bmatrix} \text{row}_1 \\ \text{row}_2 \\ \text{row}_1 + \text{row}_2 \end{bmatrix} \quad AX = b \rightarrow \begin{bmatrix} \text{row}_1 \\ \text{row}_2 \\ \text{row}_1 + \text{row}_2 \end{bmatrix} \begin{bmatrix} x_1 \\ x_2 \\ x_3 \end{bmatrix} = \begin{bmatrix} b_1 \\ b_2 \\ b_3 \end{bmatrix}$

$$b \rightarrow \begin{bmatrix} b_1 \\ b_2 \\ b_1 + b_2 \end{bmatrix}$$

$$\text{row}_1 \cdot x_1 = b_1$$

$$\text{row}_2 \cdot x_2 = b_2$$

$$\text{row}_1 \cdot x_1 + \text{row}_2 \cdot x_2 = b_3$$

c. In elimination

$$\hookrightarrow A = \begin{bmatrix} \text{row}_1 \\ \text{row}_2 \\ \text{row}_1 + \text{row}_2 \end{bmatrix} \xrightarrow{\text{Ex.}} \begin{bmatrix} \text{row}_1 \\ \text{row}_2 - \text{row}_1 \\ \text{row}_1 + \text{row}_2 \end{bmatrix} \xrightarrow{E_2} \begin{bmatrix} \text{row}_1 \\ \text{row}_2 - \text{row}_1 \\ \text{row}_1 + \text{row}_2 - \text{row}_1 \end{bmatrix} \xrightarrow{E_3} \begin{bmatrix} \text{row}_1 \\ \text{row}_2 - \text{row}_1 \\ \text{row}_1 + \text{row}_2 - \text{row}_1 - \text{row}_2 \end{bmatrix}$$

$$\text{row}_3 = \text{row}_1 - \text{row}_1 + \text{row}_2 - \text{row}_2 = 0$$

$$2) \begin{bmatrix} a & b \\ c & d \end{bmatrix} \begin{bmatrix} d & -b \\ -c & a \end{bmatrix} = \begin{bmatrix} ad - bc & -ab + ab \\ cd - cd & -bc + ad \end{bmatrix}$$

$$\text{inverse} \rightarrow \begin{bmatrix} a & -b \\ -c & d \end{bmatrix}^{-1} = \frac{1}{ad - bc} \begin{bmatrix} d & -b \\ -c & a \end{bmatrix}$$

$$\begin{bmatrix} d & -b \\ -c & a \end{bmatrix} = \frac{1}{ad - bc} \begin{bmatrix} a & b \\ c & d \end{bmatrix}$$

3) If B is the inverse of A^2 show that AB is the inverse of A

$$B = (A \cdot A)^{-1} \rightarrow (A \cdot A)B = I$$

$$A(AB) = I$$

$$A \cdot A^{-1} = I \rightarrow AB = A^{-1}$$

so AB is the inverse of A

4) $A = \begin{bmatrix} 1 & 1 & 1 \\ 1 & 2 & 2 \\ 1 & 2 & 3 \end{bmatrix}$ inverse matrix A by Gauss Jordan method starting with $[AI]$

$$\hookrightarrow \begin{bmatrix} 1 & 1 & 1 & 0 & 0 \\ 1 & 2 & 2 & 0 & 1 \\ 1 & 2 & 3 & 0 & 0 \end{bmatrix} \xrightarrow{r_2 - r_1} \begin{bmatrix} 1 & 1 & 1 & 0 & 0 \\ 0 & 1 & 1 & 0 & 1 \\ 1 & 2 & 3 & 0 & 0 \end{bmatrix} \xrightarrow{r_3 - r_1} \begin{bmatrix} 1 & 1 & 1 & 0 & 0 \\ 0 & 1 & 1 & 0 & 1 \\ 0 & 1 & 2 & 0 & 0 \end{bmatrix} \xrightarrow{r_3 - r_2} \begin{bmatrix} 1 & 1 & 1 & 0 & 0 \\ 0 & 1 & 1 & 0 & 1 \\ 0 & 0 & 1 & 0 & -1 \end{bmatrix} \xrightarrow{r_1 - r_2} \begin{bmatrix} 1 & 0 & 2 & 0 & -1 \\ 0 & 1 & 1 & 0 & 1 \\ 0 & 0 & 1 & 0 & -1 \end{bmatrix} \xrightarrow{r_2 - r_3} \begin{bmatrix} 1 & 0 & 2 & 0 & -1 \\ 0 & 1 & 0 & 0 & 2 \\ 0 & 0 & 1 & 0 & -1 \end{bmatrix}$$

$$\text{so } A^{-1} \text{ is } \begin{bmatrix} 2 & -1 & 0 \\ -1 & 2 & -1 \\ 0 & -1 & 1 \end{bmatrix}$$

5) a. Prove that $A = \begin{bmatrix} a & b & b \\ a & a & b \\ a & a & a \end{bmatrix}$ is invertible if $a \neq 0$ and $a \neq b$

elimination

$$R_2 \rightarrow R_2 - R_1 = \begin{bmatrix} 0 & a-b & 0 \end{bmatrix}$$

$$R_3 \rightarrow R_3 - R_1 = \begin{bmatrix} 0 & a-b & a-b \end{bmatrix}$$

$$R_3 \rightarrow R_3 - R_2 = \begin{bmatrix} 0 & 0 & a-b \end{bmatrix}$$

b. $C = \begin{bmatrix} 2 & c & c \\ c & c & c \\ 8 & 7 & c \end{bmatrix}, c=0$

$$= 2 \begin{bmatrix} c & c \\ 7 & c \end{bmatrix} - c \begin{bmatrix} c & c \\ 8 & c \end{bmatrix} + c \begin{bmatrix} c & c \\ 8 & 7 \end{bmatrix}$$

$$= 2(c^2 - 7c) - c(c^2 - 8c) + c(7c - 8c)$$

$$= 2c^2 - 14c - c^3 + 8c^2 - c^2$$

$$= -c^3 + 9c^2 - 14c$$

$$= -c(c^2 - 9c - 14)$$

$$= -c(c-2)(c-7)$$

$c=0 \quad c=2 \quad c=7$

Assignment 2.6

1) $A = \begin{bmatrix} 2 & 1 & 0 \\ 0 & 4 & 2 \\ 6 & 3 & 5 \end{bmatrix}$ a. $A \rightarrow$ upper triangular

$$\begin{bmatrix} 2 & 1 & 0 \\ 0 & 4 & 2 \\ 6 & 3 & 5 \end{bmatrix} \xrightarrow{r_3 - 3r_1} \begin{bmatrix} 2 & 1 & 0 \\ 0 & 4 & 2 \\ 0 & 0 & 5 \end{bmatrix}$$

b. Find matrix E such $EA=U$

$E_{31} \cdot A = U$ • Pivot = 2
• Multiplier = $q_{31} = 6/2 = 3$

$$E = E_{31} = \begin{bmatrix} 1 & 0 & 0 \\ 0 & 1 & 0 \\ -3 & 0 & 1 \end{bmatrix}$$

c. $L = E_{31}^{-1} = E^{-1} \rightarrow L = \begin{bmatrix} 1 & 0 & 0 \\ 0 & 1 & 0 \\ 3 & 0 & 1 \end{bmatrix}$

$$\left. \begin{array}{l} EA = U \\ E^{-1} \cdot EA = E^{-1} \cdot U \\ I \cdot A = LU = A \end{array} \right\}$$

3) b. Solve $UX=C$ to find x

$$\begin{bmatrix} 1 & 1 & 1 \\ 0 & 1 & 1 \\ 0 & 0 & 1 \end{bmatrix} \begin{bmatrix} x_1 \\ x_2 \\ x_3 \end{bmatrix} = \begin{bmatrix} 4 \\ 1 \\ 1 \end{bmatrix}$$

$x_3 = 1$
 $x_2 = 1 - 1 = 0$
 $x_1 = 4 - 0 - 1 = 3$

$$x = \begin{bmatrix} 3 \\ 0 \\ 1 \end{bmatrix}$$

c. $A=LU$

$$A = \begin{bmatrix} 1 & 0 & 0 \\ 1 & 1 & 0 \\ 1 & 1 & 1 \end{bmatrix} \begin{bmatrix} 1 & 1 & 1 \\ 0 & 1 & 1 \\ 0 & 0 & 1 \end{bmatrix} = \begin{bmatrix} 1 & 1 & 1 \\ 1 & 2 & 2 \\ 1 & 2 & 3 \end{bmatrix}$$

* $LC=b$

$$\begin{bmatrix} 1 & 1 & 1 \\ 1 & 2 & 2 \\ 1 & 2 & 3 \end{bmatrix} \begin{bmatrix} 4 \\ 1 \\ 1 \end{bmatrix} = \begin{bmatrix} 4 \\ 5 \\ 6 \end{bmatrix}$$

$L(Ux)=b$

$(LU)x=b$

$Ax=b$

2) $A = \begin{bmatrix} a & a & a & a \\ a & b & b & b \\ a & b & c & c \\ a & b & c & d \end{bmatrix}$ Compute L & U such that $A=LU$

$$\begin{array}{l} E_{21}, E_{31}, E_{41} \\ R_2 - R_1, R_3 - R_1, R_4 - R_1 \end{array} \rightarrow \begin{bmatrix} a & a & a & a \\ 0 & b-a & b-a & b-a \\ 0 & b-a & c-a & c-a \\ 0 & b-a & c-a & d-a \end{bmatrix} \xrightarrow{\begin{array}{l} E_{32}, E_{42} \\ R_3 - R_2, R_4 - R_2 \end{array}} \begin{bmatrix} a & a & a & a \\ 0 & b-a & b-a & b-a \\ 0 & 0 & (c-a)-(b-a) & (c-a)-(b-a) \\ 0 & 0 & (c-a)-(b-a) & (d-a)-(b-a) \end{bmatrix}$$

$$\xrightarrow{\begin{array}{l} E_{43} \\ R_4 - R_3 \end{array}} \begin{bmatrix} a & a & a & a \\ 0 & b-a & b-a & b-a \\ 0 & 0 & (c-a)-(b-a) & (c-a)-(b-a) \\ 0 & 0 & 0 & (d-a)-(c-a) \end{bmatrix} = \begin{bmatrix} a & a & a & a \\ 0 & b-a & b-a & b-a \\ 0 & 0 & c-b & c-b \\ 0 & 0 & 0 & d-c \end{bmatrix}$$

$$E_{43} E_{42} E_{32} E_{41} E_{31} E_{21} = \begin{bmatrix} 1 & 0 & 0 & 0 \\ -1 & 1 & 0 & 0 \\ -1 & 1 & 1 & 0 \\ -1 & 1 & 1 & 1 \end{bmatrix} \rightarrow L = E^{-1} = \begin{bmatrix} 1 & 0 & 0 & 0 \\ 1 & 1 & 0 & 0 \\ 1 & 1 & 1 & 0 \\ 1 & 1 & 1 & 1 \end{bmatrix}$$

3) $L = \begin{bmatrix} 1 & 0 & 0 \\ 1 & 1 & 0 \\ 1 & 1 & 1 \end{bmatrix} \quad U = \begin{bmatrix} 1 & 1 & 1 \\ 0 & 1 & 1 \\ 0 & 0 & 1 \end{bmatrix} \quad b = \begin{bmatrix} 4 \\ 5 \\ 6 \end{bmatrix}$

a. Solve $Lc=b$ to find c

$$\begin{bmatrix} 1 & 0 & 0 \\ 1 & 1 & 0 \\ 1 & 1 & 1 \end{bmatrix} \begin{bmatrix} c_1 \\ c_2 \\ c_3 \end{bmatrix} = \begin{bmatrix} 4 \\ 5 \\ 6 \end{bmatrix} \quad * c = L^{-1}b$$

$$L^{-1} \rightarrow \begin{bmatrix} 1 & 0 & 0 & 1 & 0 & 0 \\ 1 & 1 & 0 & 0 & 1 & 0 \\ 1 & 1 & 1 & 0 & 0 & 1 \end{bmatrix} \rightarrow \begin{bmatrix} 1 & 0 & 0 & 1 & 0 & 0 \\ 0 & 1 & 0 & -1 & 1 & 0 \\ 0 & 0 & 1 & 0 & 0 & 1 \end{bmatrix}$$

$$\rightarrow \begin{bmatrix} 1 & 0 & 0 & 1 & 0 & 0 \\ 0 & 1 & 0 & -1 & 1 & 0 \\ 0 & 0 & 1 & 0 & 0 & 1 \end{bmatrix} \rightarrow \begin{bmatrix} 1 & 0 & 0 & 1 & 0 & 0 \\ 0 & 1 & 0 & -1 & 1 & 0 \\ 0 & 0 & 1 & 0 & 0 & 1 \end{bmatrix}, \quad c = \begin{bmatrix} 1 & 0 & 0 \\ -1 & 1 & 0 \\ 0 & -1 & 1 \end{bmatrix} \begin{bmatrix} 4 \\ 5 \\ 6 \end{bmatrix} = \begin{bmatrix} 4 \\ 1 \\ 1 \end{bmatrix}$$

Assignment 2.7

1) $A = \begin{bmatrix} 1 & 0 \\ 0 & 3 \end{bmatrix}$ $A^T = \begin{bmatrix} 1 & 0 \\ 0 & 3 \end{bmatrix}$ $A^{-1} = \frac{1}{3-0} \begin{bmatrix} 3 & 0 \\ -0 & 1 \end{bmatrix} = \begin{bmatrix} 1 & 0 \\ -3 & 1 \end{bmatrix}$

$\cdot (A^T)^{-1} = \frac{1}{3-0} \begin{bmatrix} 3 & -0 \\ 0 & 1 \end{bmatrix} = \begin{bmatrix} 1 & -3 \\ 0 & 1 \end{bmatrix}$ } so $(A^T)^{-1} = (A^{-1})^T$
 $\cdot (A^{-1})^T = \begin{bmatrix} 1 & -3 \\ 0 & 1 \end{bmatrix}$

2) $A = \begin{bmatrix} 1 & 0 \\ 2 & 1 \end{bmatrix}$ $B = \begin{bmatrix} 1 & 3 \\ 0 & 1 \end{bmatrix}$

$\cdot A^T = \begin{bmatrix} 1 & 2 \\ 0 & 1 \end{bmatrix}$ $\cdot B^T = \begin{bmatrix} 1 & 0 \\ 3 & 1 \end{bmatrix}$ $\cdot AB = \begin{bmatrix} 1 & 3 \\ 2 & 7 \end{bmatrix}$ $\cdot (AB)^T = \begin{bmatrix} 1 & 2 \\ 3 & 7 \end{bmatrix}$

$\cdot B^T A^T = \begin{bmatrix} 1 & 0 \\ 3 & 1 \end{bmatrix} \begin{bmatrix} 1 & 2 \\ 0 & 1 \end{bmatrix} = \begin{bmatrix} 1 & 2 \\ 3 & 7 \end{bmatrix} = (AB)^T$

$\cdot A^T B^T = \begin{bmatrix} 1 & 2 \\ 0 & 1 \end{bmatrix} \begin{bmatrix} 1 & 0 \\ 3 & 1 \end{bmatrix} = \begin{bmatrix} 7 & 2 \\ 3 & 1 \end{bmatrix} \neq (AB)^T$

3) $S = \begin{bmatrix} 2 & -1 & 0 \\ -1 & 2 & -1 \\ 0 & -1 & 2 \end{bmatrix}$ factor into $S = LDL^T$ w/ diagonal pivot matrix D

$\cdot S = L U \xrightarrow[r_{21} = -1/2]{r_2 + 1/2 r_1} \begin{bmatrix} 2 & -1 & 0 \\ 0 & 3/2 & -1 \\ 0 & -1 & 2 \end{bmatrix} \xrightarrow[l_{32} = -2/3]{r_3 + 2/3 r_2} \begin{bmatrix} 2 & -1 & 0 \\ 0 & 3/2 & -1 \\ 0 & 0 & 4/3 \end{bmatrix}$ $\cdot E = E_{32} E_{21} = \begin{bmatrix} 1 & 0 & 0 \\ 1/2 & 1 & 0 \\ 0 & 2/3 & 1 \end{bmatrix}$

$\cdot L = E^{-1} = \begin{bmatrix} 1 & 0 & 0 \\ -1/2 & 1 & 0 \\ 0 & -2/3 & 1 \end{bmatrix} \longrightarrow S = LDL^T \rightarrow \begin{bmatrix} 1 & 0 & 0 \\ -1/2 & 1 & 0 \\ 0 & -2/3 & 1 \end{bmatrix} \begin{bmatrix} 2 & 0 & 0 \\ 0 & 3/2 & 0 \\ 0 & 0 & 4/3 \end{bmatrix} \begin{bmatrix} 1 & -1/2 & 0 \\ 0 & 1 & -2/3 \\ 0 & 0 & 1 \end{bmatrix}$
 $\cdot U = \begin{bmatrix} 1 & -1/2 & 0 \\ 0 & 1 & -2/3 \\ 0 & 0 & 1 \end{bmatrix}$

4) $A = \begin{bmatrix} 0 & 1 & 1 \\ 1 & 0 & 1 \\ 2 & 3 & 4 \end{bmatrix}$ find the factorization
 $PA = LU$

$PA \rightarrow \begin{bmatrix} 0 & 1 & 1 \\ 1 & 0 & 1 \\ 0 & 0 & 1 \end{bmatrix} \begin{bmatrix} 0 & 1 & 1 \\ 1 & 0 & 1 \\ 2 & 3 & 4 \end{bmatrix} = \begin{bmatrix} 1 & 0 & 1 \\ 0 & 1 & 1 \\ 2 & 3 & 4 \end{bmatrix}$

$L U \rightarrow$

$\begin{bmatrix} 1 & 0 & 1 \\ 0 & 1 & 1 \\ 2 & 3 & 4 \end{bmatrix} \xrightarrow[l_{31} = 2]{r_3 - 2r_1} \begin{bmatrix} 1 & 0 & 1 \\ 0 & 1 & 1 \\ 0 & 3 & 2 \end{bmatrix} \xrightarrow[l_{32} = 3]{r_3 - 3r_2} \begin{bmatrix} 1 & 0 & 1 \\ 0 & 1 & 1 \\ 0 & 0 & -1 \end{bmatrix} = U$

$E = E_{32} \cdot E_{31} = \begin{bmatrix} 1 & 0 & 0 \\ 0 & 1 & 0 \\ -2 & -3 & 1 \end{bmatrix}$ $L = E^{-1} = \begin{bmatrix} 1 & 0 & 0 \\ 0 & 1 & 0 \\ 2 & 3 & 1 \end{bmatrix}$

$PA = LU$
 $\begin{bmatrix} 0 & 1 & 1 \\ 1 & 0 & 1 \\ 0 & 0 & 1 \end{bmatrix} \begin{bmatrix} 0 & 1 & 1 \\ 1 & 0 & 1 \\ 2 & 3 & 4 \end{bmatrix} = \begin{bmatrix} 1 & 0 & 1 \\ 0 & 1 & 1 \\ 2 & 3 & 1 \end{bmatrix} \begin{bmatrix} 1 & 0 & 1 \\ 0 & 1 & 1 \\ 0 & 0 & -1 \end{bmatrix}$

Assignment 3.1

1) $\det Q = \begin{vmatrix} \cos \theta & -\sin \theta \\ \sin \theta & \cos \theta \end{vmatrix}$

$\det Q = \frac{1}{\cos^2 \theta + \sin^2 \theta} = \frac{1}{1} = 1$

2) $A = \begin{bmatrix} 4 & 1 \\ 2 & 3 \end{bmatrix}$ $\cdot A^2 = \begin{bmatrix} 4 & 1 \\ 2 & 3 \end{bmatrix} \begin{bmatrix} 4 & 1 \\ 2 & 3 \end{bmatrix} = \begin{bmatrix} 18 & 7 \\ 14 & 11 \end{bmatrix}$ $\cdot \det A^2 = \frac{1}{198 - 98} = \frac{1}{100}$

$\cdot A^{-1} = \frac{1}{12 - 2} \begin{bmatrix} 3 & -1 \\ -2 & 4 \end{bmatrix} = \begin{bmatrix} 3/10 & -1/10 \\ -2/10 & 4/10 \end{bmatrix}$ $\cdot \det A^{-1} = \frac{1}{\frac{12}{100} - \frac{2}{100}} = 1 \cdot \frac{10}{100} = 10$

$$3) A = \begin{bmatrix} 0 & 1 & 1 \\ 1 & 0 & 1 \\ 1 & 1 & 0 \end{bmatrix} \rightarrow \det A = ?$$

$$\hookrightarrow \begin{bmatrix} 0 & 1 & 1 \\ 1 & 0 & 1 \\ 1 & 1 & 0 \end{bmatrix} \begin{matrix} 0 & 1 \\ 1 & 0 \\ 1 & 1 \end{matrix} \det A = 0 + 1 + 1 - 0 - 0 - 0 = 2$$

4) apply row operations to produce an upper triangular U

$$\begin{bmatrix} 1 & 2 & 3 & 0 \\ 2 & 6 & 6 & 1 \\ -1 & 0 & 0 & 3 \\ 0 & 2 & 0 & 7 \end{bmatrix} \xrightarrow{r_2 - 2r_1} \begin{bmatrix} 1 & 2 & 3 & 0 \\ 0 & 2 & 0 & 1 \\ -1 & 0 & 0 & 3 \\ 0 & 2 & 0 & 7 \end{bmatrix} \xrightarrow{r_3 + r_1} \begin{bmatrix} 1 & 2 & 3 & 0 \\ 0 & 2 & 0 & 1 \\ 0 & 2 & 3 & 3 \\ 0 & 2 & 0 & 7 \end{bmatrix}$$

$$\begin{matrix} r_3 - r_2 \\ r_4 - r_2 \end{matrix} \rightarrow \begin{bmatrix} 1 & 2 & 3 & 0 \\ 0 & 2 & 0 & 1 \\ 0 & 0 & 3 & 2 \\ 0 & 0 & 0 & 6 \end{bmatrix}$$

$$\det \begin{bmatrix} 1 & 2 & 3 & 0 \\ 0 & 2 & 0 & 1 \\ 0 & 0 & 3 & 2 \\ 0 & 0 & 0 & 6 \end{bmatrix} \rightarrow 1 \cdot 2 \cdot 3 \cdot 6 + 0 + 0 + 0 - 0 - 0 - 0 - 0 = 36$$